WIP: RangeTreeBag

src/QueryStructure/Specification/SearchTerms/InRange.v
@@ -1,20 +1,40 @@
 Require Import Coq.Arith.Compare_dec Omega
         Fiat.QueryStructure.Specification.Representation.QueryStructureNotations.
 
-Section RangeClause.  
-  Definition InRange (n : nat) (range : nat * nat) :=
-    (fst range) <= n <= (snd range).
+Section RangeClause.
+  Definition InRange (n : nat) (range : (option nat) * (option nat)) :=
+    match range with
+      | (None        , None        ) => True
+      | (Some min_key, None        ) => min_key <= n
+      | (None        , Some max_key) => n <= max_key
+      | (Some min_key, Some max_key) => min_key <= n <= max_key
+    end.
 
-  Definition InRange_dec (n : nat) (range : nat * nat)
+  Definition InRange_dec (n : nat) (range : option nat * option nat)
   : {InRange n range} + {~ InRange n range}.
     refine (
-        if le_dec (fst range) n then
-          if le_dec n (snd range) then
+        match range with
+          | (None        , None        ) =>
             left _
-          else
-            right _
-        else
-          right _); unfold InRange in *; intuition eauto.
+          | (Some min_key, None        ) =>
+            if le_dec min_key n then
+              left _
+            else
+              right _
+          | (None        , Some max_key) =>
+            if le_dec n max_key then
+              left _
+            else
+              right _
+          | (Some min_key, Some max_key) =>
+            if le_dec min_key n then
+              if le_dec n max_key then
+                left _
+              else
+                right _
+            else
+              right _
+        end); unfold InRange in *; intuition eauto.
   Defined.
 
   Global Instance DecideableEnsemble_InRange st :
