src/QueryStructure/Automation/SearchTerms/RangeSearchTerms.v
@@ -13,7 +13,7 @@ Definition RangeIndex : string := "RangeIndex".
 Record RangeSearchTerm
        (heading : Heading)
   :=
-    { RangeIndexSearchTerm : option (nat * nat);
+    { RangeIndexSearchTerm : ((option nat) * (option nat));
       RangeItemSearchTerm : @Tuple heading -> bool }.
 
 (* This builds the type of searchterms and the matching function on them *)
@@ -24,14 +24,12 @@ Global Instance RangeIndexDenotation
 : @IndexDenotation "RangeIndex" heading index :=
   {| DenoteIndex := RangeSearchTerm heading; (* Pick search term type *)
      MatchIndex search_term item := (* matching function : DenoteIndex -> Tuple heading -> bool *)
-       match RangeIndexSearchTerm search_term with
-         | Some indexSearchTerm =>
-           if InRange_dec (projection item) indexSearchTerm then
-             RangeItemSearchTerm search_term item
-           else false
-         | None =>
-           RangeItemSearchTerm search_term item
-       end |}.
+       if InRange_dec (projection item) (RangeIndexSearchTerm search_term) then
+         RangeItemSearchTerm search_term item
+       else
+         false |}.
+
+(* TODO: All tactics below this need to be updated to the new definition on RangeSearchTerm *)
 
 (* Extra type class magic for range indices. *)
 Hint Extern 10 (@IndexDenotation "RangeIndex" ?heading ?index) =>
